x86/TablesEncodeproof.v
@@ -30,28 +30,49 @@ Variables prog tprog: RelocProgram.program.
 
 Hypothesis transf_encode: TablesEncode.transf_program prog = OK tprog.
 
-Hypothesis valid_reloctables:
+Lemma valid_reloctables:
   forall id, Forall valid_relocentry (get_reloctable id (prog_reloctables prog)).
+Proof.
+  unfold transf_program in transf_encode.
+  monadInv transf_encode. repeat destr_in EQ0.
+Qed.
 
-Hypothesis valid_symbentries_p:
-  forall strmap sbytes,
-    get_strings_map_bytes (fold_right acc_symbols nil (prog_symbtable prog)) = OK (strmap, sbytes) ->
+Lemma valid_symbentries_p:
+  forall strmap sbytes idbytes,
+    get_strings_map_bytes (fold_right acc_symbols nil (prog_symbtable prog)) = OK (idbytes, strmap, sbytes) ->
     Forall (valid_symbentry strmap) (RelocProgram.prog_symbtable prog).
+Proof.
+  unfold transf_program in transf_encode.
+  monadInv transf_encode. repeat destr_in EQ0.
+Qed.
 
-Hypothesis empty_strtable:
+Lemma empty_strtable:
   prog_strtable prog = Maps.PTree.empty Z.
+Proof.
+  unfold transf_program in transf_encode.
+  monadInv transf_encode. repeat destr_in EQ0.
+Qed.
 
-Hypothesis symbentries_no_repet:
+Lemma symbentries_no_repet:
   list_norepet (map symbentry_id (prog_symbtable prog)).
+Proof.
+  unfold transf_program in transf_encode.
+  monadInv transf_encode. repeat destr_in EQ0.
+Qed.
 
-Parameter prog_strings : list (ident * list byte).
-Hypothesis prog_strings_eq:
-  fold_right acc_symbol_strings (OK [])
-             (fold_right acc_symbols [] (prog_symbtable prog)) =
-  OK prog_strings.
-
-Hypothesis prog_strings_not_empty:
-  Forall (fun '(_, lb) => lb <> []) prog_strings.
+Lemma prog_strings_eq:
+  forall l idbytes strmap sbytes,
+    get_strings_map_bytes l = OK (idbytes, strmap, sbytes) ->
+    Forall (fun '(_, lb) => lb <> []) idbytes.
+Proof.
+  intros.
+  unfold get_strings_map_bytes in H. monadInv H. repeat destr_in EQ0.
+  clear Heqp. revert l idbytes EQ. induction l; simpl; intros; eauto.
+  inv EQ; auto.
+  unfold acc_symbol_strings in EQ at 1. monadInv EQ. repeat destr_in EQ1.
+  constructor; eauto. intro EQm; apply (f_equal (@length _)) in EQm.
+  rewrite app_length in EQm; simpl in EQm. omega.
+Qed.
 
 
 Lemma acc_symbols_in_in_symbols:
@@ -73,16 +94,16 @@ Proof.
 Qed.
 
 Lemma gsmb_valid_strtable:
-  forall pi strmap sbytes,
+  forall pi strmap sbytes idbytes,
          let symbols := fold_right acc_symbols [] (prog_symbtable pi) in
-         get_strings_map_bytes symbols = OK (strmap, sbytes) ->
+         get_strings_map_bytes symbols = OK (idbytes, strmap, sbytes) ->
          forall
          x (EQ0 : fold_right acc_symbol_strings (OK []) (fold_right acc_symbols [] (prog_symbtable pi)) = OK x)
          (LNR: list_norepet (map symbentry_id (prog_symbtable pi)))
 ,
     valid_strtable x strmap.
 Proof.
-  intros pi strmap sbytes symbols GSMB x EQ0 LNR.
+  intros pi strmap sbytes idbytes symbols GSMB x EQ0 LNR.
   unfold valid_strtable.
 
   assert (LNR': list_norepet (map fst x)).
@@ -105,7 +126,7 @@ Proof.
   unfold symbols in GSMB. rewrite EQ0 in GSMB. simpl in GSMB. repeat destr_in GSMB.
   exists z; split; auto.
   revert z Heqp l.
-  assert (valid_strtable_thr x (Maps.PTree.empty Z) 1 /\ 0 < 1).
+  assert (valid_strtable_thr idbytes (Maps.PTree.empty Z) 1 /\ 0 < 1).
   {
     split.
     constructor; setoid_rewrite Maps.PTree.gempty; congruence.
@@ -116,13 +137,13 @@ Proof.
   revert VALID POS.
   generalize (Maps.PTree.empty Z) 1.
   clear -LNR'.
-  assert (forall elt, In elt x -> In elt x) by auto. revert H.
-  generalize x at 1 4.
-  induction x0; simpl.
+  assert (forall elt, In elt idbytes -> In elt idbytes) by auto. revert H.
+  generalize idbytes at 1 4.
+  induction idbytes0; simpl.
   - intros; eauto. inv Heqp. auto.
   - intros IN t z VALID POS t0 z1 FOLD LT.
     destr_in FOLD.
-    eapply IHx0 in FOLD. auto. eauto.
+    eapply IHidbytes0 in FOLD. auto. eauto.
     constructor; repeat setoid_rewrite Maps.PTree.gsspec.
     + intros i0 j x1 y bytesx bytesy ox oy. repeat destr.
       * intros Tx Ty Bx By Diff Ox Oy. inv Tx. inv VALID.
@@ -150,11 +171,14 @@ Proof.
 Qed.
 
 Lemma valid_strtable_p:
-  forall strmap sbytes,
-    get_strings_map_bytes (fold_right acc_symbols nil (prog_symbtable prog)) = OK (strmap, sbytes) ->
-    valid_strtable prog_strings strmap.
+  forall strmap sbytes idbytes,
+    get_strings_map_bytes (fold_right acc_symbols nil (prog_symbtable prog)) = OK (idbytes, strmap, sbytes) ->
+    valid_strtable idbytes strmap.
 Proof.
   intros. eapply gsmb_valid_strtable; eauto.
+  unfold get_strings_map_bytes in H. monadInv H.
+  repeat destr_in EQ0.
+  eapply symbentries_no_repet.
 Qed.
 
 Lemma tables_encode_spec:
@@ -167,9 +191,9 @@ Lemma tables_encode_spec:
     prog_reloctables prog = prog_reloctables tprog /\
     prog_senv prog = prog_senv tprog /\
     length (prog_sectable prog) = 2%nat /\
-    exists (strmap : Maps.PTree.t Z) (sbytes : list byte) symt,
+    exists (strmap : Maps.PTree.t Z) (sbytes : list byte) idbytes symt,
       get_strings_map_bytes (fold_right acc_symbols nil (prog_symbtable prog)) =
-      OK (strmap, sbytes) /\
+      OK (idbytes, strmap, sbytes) /\
       create_symbtable_section strmap (prog_symbtable prog) = OK symt /\
       prog_strtable tprog = strmap /\
       prog_sectable tprog =
@@ -190,7 +214,7 @@ Proof.
     apply beq_nat_true in Heqb. rewrite app_length in Heqb.
     simpl in Heqb. omega.
   }
-  rewrite EQ. exists t, l, x. auto.
+  rewrite EQ. exists t, l, l0, x. auto.
 Qed.
 
 Lemma genv_senv_same:
@@ -212,7 +236,8 @@ Proof.
   unfold RelocProgSemantics1.globalenv. simpl.
   unfold RelocProgSemantics.globalenv.
   exploit tables_encode_spec; eauto.
-  intros (EQdefs & EQpublic & EQmain & EQsymt & EQreloct & EQsenv & LEN & strmap & sbytes & symt
+  intros (EQdefs & EQpublic & EQmain & EQsymt & EQreloct & EQsenv & LEN
+          & strmap & sbytes & idbytes & symt
           & GSMB & CSS & EQstrt & EQsect).
   f_equal; try intuition congruence.
   f_equal; try intuition congruence.
@@ -231,7 +256,7 @@ Proof.
   unfold RelocProgSemantics1.globalenv. simpl.
   unfold RelocProgSemantics1.gen_reloc_ofs_symbs.
   exploit tables_encode_spec; eauto.
-  intros (EQdefs & EQpublic & EQmain & EQsymt & EQreloct & EQsenv & strmap & sbytes & symt
+  intros (EQdefs & EQpublic & EQmain & EQsymt & EQreloct & EQsenv & strmap & sbytes & idbytes & symt
           & GSMB & CSS & EQstrt & EQsect).
   f_equal; try intuition congruence.
 Qed.
@@ -249,8 +274,10 @@ Lemma decode_tables_correct:
   decode_tables tprog = OK prog.
 Proof.
   exploit tables_encode_spec; eauto.
-  intros (EQdefs & EQpublic & EQmain & EQsymt & EQreloct & EQsenv & LEN & strmap & sbytes & symt
+  intros (EQdefs & EQpublic & EQmain & EQsymt & EQreloct & EQsenv & LEN
+          & strmap & sbytes & idbytes & symt
           & GSMB & CSS & EQstrt & EQsect).
+  generalize empty_strtable. intro EMP.
   unfold decode_tables.
   rewrite EQsect.
   destruct (prog_sectable prog) eqn:?; simpl in LEN; try omega.
@@ -264,8 +291,9 @@ Proof.
   erewrite decode_create_symtable_section. 5: eauto. simpl.
   destruct prog; simpl in *. subst. f_equal. f_equal; intuition try congruence.
   destruct tprog; simpl. destruct prog_reloctables; simpl; auto.
-  all: eauto.
   eapply valid_strtable_p; eauto.
+  eapply prog_strings_eq; eauto.
+  eapply valid_symbentries_p; eauto.
   apply valid_reloctables with (id := RELOC_CODE).
   apply valid_reloctables with (id := RELOC_DATA).
 Qed.
@@ -300,6 +328,501 @@ Proof.
   auto. auto. auto.
 Defined.
 
+Require Import Lia.
+
+Lemma SecTable_gsspec':
+  forall (i j : nat) (tbl : SecTable.t) (tbl' : list SecTblParams.V) (v : SecTblParams.V),
+    SecTable.set_nat i v tbl = Some tbl' ->
+    nth_error tbl' j = if Nat.eq_dec i j then Some v else nth_error tbl j.
+Proof.
+  induction i; simpl; intros; eauto.
+  - repeat destr_in H. destr.
+    + subst; reflexivity.
+    + destruct j; simpl; auto. congruence.
+  - repeat destr_in H.
+    generalize (IHi i _ _ _ Heqo). intro EQ1.
+    destr. subst; simpl. rewrite EQ1. destr.
+    destruct j. reflexivity. simpl.
+    erewrite IHi. destr. eauto.
+Qed.
+
+Lemma SecTable_gsspec:
+  forall i j tbl tbl' v,
+    (j >= SecTblParams.ofs)%N ->
+    (i >= SecTblParams.ofs)%N ->
+    SecTable.set i v tbl = Some tbl' ->
+    SecTable.get j tbl' = if N.eq_dec i j then Some v else SecTable.get j tbl.
+Proof.
+  unfold SecTable.set, SecTable.get.
+  intros.
+  erewrite SecTable_gsspec'. 2: eauto.
+  destr.
+  - apply Nnat.N2Nat.inj in e.
+    unfold SecTable.idx in e.
+    destr.
+    apply f_equal with (f:= fun x => N.add x SecTblParams.ofs) in e.
+    rewrite <- ! N.add_sub_swap in e by lia.
+    rewrite !N.add_sub in e. congruence.
+  - destr.
+Qed.
+
+Lemma remove_first_n_length:
+  forall {A} n (l l': list A),
+    RelocBinDecode.remove_first_n l n = OK l' ->
+    length l = (length l' + n)%nat.
+Proof.
+  induction n; simpl; intros; eauto. inv H. lia.
+  repeat destr_in H. simpl. apply IHn in H1. lia.
+Qed.
+
+Ltac autoinv :=
+  repeat match goal with
+         | H: context [match ?a with _ => _ end] |- _ =>
+           repeat destr_in H
+         | H: bind _ _ = OK _ |- _ =>
+           monadInv H
+         end.
+
+Opaque Z.of_nat Z.add.
+Transparent Asm.addrmode_size.
+
+Lemma decode_addrmode_SIB_size:
+  forall rom ofs sib mod_b mc am mc',
+    RelocBinDecode.addrmode_parse_SIB rom ofs sib mod_b mc = OK (am, mc') ->
+    let idx := ( Byte.shru (Byte.and sib (Byte.repr 56)) (Byte.repr 3)) in
+    let ss :=  (Byte.shru sib (Byte.repr 6)) in
+    let bs := (Byte.and sib (Byte.repr 7)) in
+    idx <> Byte.repr 4 -> (* RSP can not be the index of SIB *)
+    (if Byte.eq_dec bs (Byte.repr 5)
+     then
+       if Byte.eq_dec mod_b (Byte.zero)
+       then 2 else 6
+     else 6
+    )
+    + Z.of_nat (length mc) = Asm.addrmode_size am + Z.of_nat (length mc').
+Proof.
+  intros rom ofs sib mod_b mc am mc' APSIB idx ss bs NORSP.
+  unfold RelocBinDecode.addrmode_parse_SIB in APSIB.
+  unfold Asm.addrmode_size.
+  fold bs ss idx in APSIB.
+  autoinv.
+  - simpl.
+    unfold RelocBinDecode.addrmode_SIB_parse_index.
+    simpl. rewrite ! Z.add_0_l.
+    rewrite pred_dec_true. 2: rewrite e0. 2: reflexivity.
+    rewrite (@ pred_dec_true (Byte.repr 0 = Byte.zero)). 2: reflexivity.
+    rewrite (@ pred_dec_false (idx = _)). 2: auto.
+    lia.
+  - simpl.
+    rewrite pred_dec_false by auto.
+    unfold RelocBinDecode.addrmode_SIB_parse_index.
+    rewrite pred_dec_false by auto. lia.
+  - simpl.
+    unfold RelocBinDecode.addrmode_SIB_parse_base in EQ2. simpl in EQ2.
+    rewrite !Z.add_0_l in *.
+    rewrite (@pred_dec_false (mod_b = Byte.zero)) in * by auto.
+    rewrite (@pred_dec_false (mod_b = Byte.repr 0)) in * by auto.
+    unfold RelocBinDecode.addrmode_SIB_parse_index.
+    rewrite (@pred_dec_false (idx = _)) by auto. destr.
+  - rewrite pred_dec_true. 2: rewrite e0; reflexivity.
+    rewrite pred_dec_true by reflexivity. simpl.
+    unfold RelocBinDecode.addrmode_SIB_parse_index.
+    rewrite (@pred_dec_false (idx = _)) by auto. lia.
+  - rewrite pred_dec_false. 2: auto.
+    simpl.
+    unfold RelocBinDecode.addrmode_SIB_parse_index.
+    rewrite (@pred_dec_false (idx = _)) by auto. lia.
+  - simpl.
+    unfold RelocBinDecode.addrmode_SIB_parse_index.
+    rewrite (@pred_dec_false (idx = _)) by auto.
+    rewrite (@pred_dec_false (mod_b = Byte.zero)) in * by auto. destr.
+Qed.
+
+Lemma decode_addrmode_size:
+  forall rom ofs l x0,
+    RelocBinDecode.decode_addrmode rom ofs l = OK x0 ->
+    Z.of_nat (length l) = Asm.addrmode_size (snd (fst x0)) + Z.of_nat (length (snd x0)).
+Proof.
+  unfold RelocBinDecode.decode_addrmode. intros.
+  unfold Asm.addrmode_size.
+  autoinv; simpl.
+  - destruct x2. exploit decode_addrmode_SIB_size. eauto. admit.
+    rewrite e. rewrite (@pred_dec_true ( _ = Byte.zero)) by reflexivity. simpl; intros.
+    unfold Asm.addrmode_size in H. rewrite <- H.
+    unfold RelocBinDecode.addrmode_parse_SIB in EQ0.
+    monadInv EQ0.
+    repeat destr_in EQ6.
+    rewrite e2. rewrite pred_dec_true; auto. lia.
+    simpl in H.
+    admit. admit. admit.
+  - lia.
+  - lia.
+  - admit.
+  - destruct x2. exploit decode_addrmode_SIB_size. eauto. admit. simpl in *. subst.
+    rewrite e. rewrite (@pred_dec_false ( _ = Byte.zero)). 2: intro A; inv A. simpl; intros.
+    unfold Asm.addrmode_size in H. admit.
+  - admit.
+  -
+Admitted.
+
+Lemma decode_instr_size:
+  forall rom symt ofs bs ins bs',
+    RelocBinDecode.fmc_instr_decode rom symt ofs bs = OK (ins, bs') ->
+    Z.of_nat (length bs) = Asm.instr_size ins + Z.of_nat (length bs').
+Proof.
+  Transparent Asm.instr_size.
+  unfold RelocBinDecode.fmc_instr_decode, Asm.instr_size.
+  intros rom symt ofs bs ins bs' DEC.
+  Ltac helper :=
+    repeat match goal with
+           | H: RelocBinDecode.remove_first_n ?l ?n = OK ?l' |- _ =>
+             rewrite (remove_first_n_length _ _ _ H)
+           | H: context [match ?a with _ => _ end] |- _ =>
+             repeat destr_in H
+           | H: bind _ _ = OK _ |- _ =>
+             monadInv H
+           | H: ?f ?l = OK (?ins: Asm.instruction, ?bs': list byte) |- _ =>
+             unfold f in H
+           | H: ?f _ _ = OK (?ins: Asm.instruction, ?bs': list byte) |- _ =>
+             unfold f in H
+           | H: ?f _ _ _ = OK (?ins: Asm.instruction, ?bs': list byte) |- _ =>
+             unfold f in H
+           | H: ?f _ _ _ _ = OK (?ins: Asm.instruction, ?bs': list byte) |- _ =>
+             unfold f in H
+           | H: ?f _ _ _ _ _ = OK (?ins: Asm.instruction, ?bs': list byte) |- _ =>
+             unfold f in H
+           | |- _ => simpl; try lia
+           end.
+  Transparent Z.of_nat.
+  repeat destr_in DEC.
+  - helper.
+  - helper.
+  - helper.
+  - helper.
+  - helper.
+    exploit decode_addrmode_size. eauto. lia.
+  - helper.
+  - helper.
+  - helper.
+  - helper.
+  - helper.
+    exploit decode_addrmode_size. eauto. lia.
+  - helper.
+    exploit decode_addrmode_size. eauto. lia.
+  - helper.
+  - helper.
+  - helper.
+    admit.
+  - helper.
+  - helper.
+  - helper.
+  - helper.
+Admitted.
+
+Lemma decode_instrs_size:
+  forall rom symt fuel bs ofs insns x1,
+    decode_instrs rom symt fuel ofs bs insns = OK x1 ->
+    Z.of_nat (length bs) + Asm.code_size (rev insns) = Asm.code_size x1.
+Proof.
+  induction fuel;  intros; eauto.
+  - simpl in H. repeat destr_in H. simpl. auto.
+  - simpl in H. destr_in H. inv H; simpl; auto.
+    monadInv H.
+    destruct x. erewrite decode_instr_size; eauto.
+    erewrite <- IHfuel with (x1 := x1); eauto.
+    simpl. rewrite AsmFacts.code_size_app. simpl. lia.
+Qed.
+
+Lemma decode_instrs'_size:
+  forall rom symt bs x1,
+    decode_instrs' rom symt bs = OK x1 ->
+    Z.of_nat (length bs) = Asm.code_size x1.
+Proof.
+  unfold decode_instrs'. intros rom symt bs x1 DEC.
+  monadInv DEC.
+  eapply decode_instrs_size in EQ. simpl in EQ. lia.
+Qed.
+
+
+Lemma fold_acc_strmap_size:
+  forall l idbytes t0 o0 t1 o1 z,
+    fold_left acc_strmap idbytes (t0, o0) = (t1, o1) ->
+    fold_right acc_symbol_strings (OK []) l = OK idbytes ->
+    fold_right (fun id acc =>
+                  match acc with
+                    OK z =>
+                    match SymbolString.find_symbol_pos id with
+                    | Some pos => OK (z + 2 + Z.of_nat (length pos))
+                    | None => Error (msg "cannot find string")
+                    end
+                  | _ => acc
+                  end
+               ) (OK 0) l = OK z ->
+    o1 + Z.of_nat (length idbytes) = o0 + z.
+Proof.
+  induction l; simpl; intros; eauto.
+  inv H0. inv H1. simpl in H. inv H. simpl. lia.
+  destr_in H1. unfold acc_symbol_strings in H0 at 1.
+  monadInv H0. destr_in H1. inv EQ0. inv H1.
+  simpl in H.
+  exploit IHl. eauto. eauto. eauto. simpl.
+  rewrite app_length. rewrite map_length. simpl. lia.
+Qed.
+
+Lemma get_strings_map_bytes_exists':
+  forall l z,
+    fold_right (fun id acc =>
+                  match acc with
+                    OK z =>
+                    match SymbolString.find_symbol_pos id with
+                    | Some pos => OK (z + 2 + Z.of_nat (length pos))
+                    | None => Error (msg "cannot find string")
+                    end
+                  | _ => acc
+                  end
+               ) (OK 0) l = OK z ->
+    z < Int.max_unsigned ->
+    exists idbytes strmap sbytes,
+      get_strings_map_bytes l = OK (idbytes, strmap, sbytes).
+Proof.
+  unfold get_strings_map_bytes.
+  induction l; simpl; intros; eauto.
+  repeat destr_in H.
+  edestruct IHl as (idbytes & strmap & sbytes & EQ). eauto. lia.
+  monadInv EQ. repeat destr_in EQ1.
+  rewrite EQ0. simpl. rewrite Heqo. simpl.
+  destr.
+  exploit fold_acc_strmap_size. eauto. eauto. eauto. intro EQ. rewrite pred_dec_true.
+  (do 3 eexists); eauto.
+  revert EQ.
+  rewrite app_length.
+  rewrite map_length. simpl. revert H0. clear.
+  intros.
+  eapply Z.le_lt_trans. 2: apply H0. lia.
+Qed.
+
+Lemma get_strings_map_bytes_exists:
+  forall syms z,
+    fold_right (fun id acc =>
+                  match acc with
+                    OK z =>
+                    match SymbolString.find_symbol_pos id with
+                    | Some pos => OK (z + 2 + Z.of_nat (length pos))
+                    | None => Error (msg "cannot find string")
+                    end
+                  | _ => acc
+                  end
+               ) (OK 0) (fold_right acc_symbols [] syms) = OK z ->
+    z < Int.max_unsigned ->
+    exists idbytes strmap sbytes,
+      get_strings_map_bytes (fold_right acc_symbols [] syms) = OK (idbytes, strmap, sbytes).
+Proof.
+  intros.
+  eapply get_strings_map_bytes_exists'; eauto.
+Qed.
+
+Lemma create_symbtable_section_succeeds:
+  forall strmap symt,
+    Forall (fun s => exists si, Maps.PTree.get (symbentry_id s) strmap = Some si) symt ->
+    exists symsec,
+      create_symbtable_section strmap symt = OK symsec.
+Proof.
+  unfold create_symbtable_section.
+  unfold encode_symbtable.
+  induction symt; simpl; intros. eauto.
+  destruct IHsymt. inv H; auto. monadInv H0. rewrite EQ. simpl.
+  unfold encode_symbentry.
+  inv H. destruct H2. rewrite H. simpl. eauto.
+Qed.
+
+Lemma link_reloc_bingen_sectable:
+  forall p1 p2 p,
+    link_reloc_bingen p1 p2 = Some p ->
+    length (prog_sectable p) = 2%nat.
+Proof.
+  unfold link_reloc_bingen.
+  intros.
+  repeat destr_in H.
+  unfold RelocBingen.transf_program in Heqr1.
+  autoinv. simpl.
+  unfold RelocBingen.transl_sectable in EQ. autoinv. reflexivity.
+Qed.
+
+
+
+Lemma get_symbtable_to_tree:
+  forall stbl,
+    (symbtable_to_tree stbl) =
+    (Maps.PTree_Properties.of_list (map (fun s =>(symbentry_id s, s)) stbl)).
+Proof.
+  reflexivity.
+Qed.
+
+Lemma symbtable_to_tree_get_id:
+  forall stbl x se,
+    Maps.PTree.get x (symbtable_to_tree stbl) = Some se ->
+    x = symbentry_id se /\ In se stbl.
+Proof.
+  intros. rewrite get_symbtable_to_tree in H.
+  apply Maps.PTree_Properties.in_of_list in H.
+  rewrite in_map_iff in H.
+  decompose [ex and] H; clear H. inv H1. auto.
+Qed.
+
+Lemma get_strings_map_bytes_in:
+  forall l idbytes strmap sbytes,
+    get_strings_map_bytes l = OK (idbytes, strmap, sbytes) ->
+    forall i si,
+      Maps.PTree.get i strmap = Some si ->
+      In i l.
+Proof.
+  unfold get_strings_map_bytes. intros. autoinv.
+
+  assert (
+      forall idbytes t0 o0 t1 o1 i si,
+        fold_left acc_strmap idbytes (t0, o0) = (t1, o1) ->
+        Maps.PTree.get i t1 = Some si ->
+        Maps.PTree.get i t0 <> None \/ In i (map fst idbytes)
+    ).
+  {
+    clear.
+    induction idbytes; simpl; intros; eauto.
+    inv H. left ; congruence.
+    destr_in H. eapply IHidbytes in H; eauto.
+    rewrite Maps.PTree.gsspec in H. destr_in H. destruct H. subst; simpl; auto. eauto.
+  }
+  edestruct H. eauto. eauto. rewrite Maps.PTree.gempty in H1. congruence.
+
+  assert (forall l b0 b1,
+             fold_right acc_symbol_strings (OK b0) l = OK b1 ->
+             forall i,
+               In i (map fst b1) ->
+               In i (map fst b0) \/ In i l
+         ).
+  {
+    clear.
+    induction l; simpl; intros; eauto.
+    inv H. auto.
+    unfold acc_symbol_strings in H at 1. autoinv. simpl in H0. destruct H0; auto.
+    eapply IHl in EQ; eauto. intuition.
+  }
+  edestruct H2; eauto. easy.
+Qed.
+
+Lemma acc_strmap_acc:
+  forall l t0 i0 t1 i1,
+    fold_left acc_strmap l (t0, i0) = (t1, i1) ->
+    forall i,
+      Maps.PTree.get i t0 <> None -> Maps.PTree.get i t1 <> None.
+Proof.
+  induction l; simpl; intros; eauto. inv H; eauto.
+  destr_in H.
+  eapply IHl in H. eauto. rewrite Maps.PTree.gsspec. destr.
+Qed.
+
+Lemma acc_strmap_exists:
+  forall l t0 i0 t1 i1 i,
+    In i (map fst l) ->
+    fold_left acc_strmap l (t0, i0) = (t1, i1) ->
+    Maps.PTree.get i t1 <> None.
+Proof.
+  induction l; simpl; intros; eauto.
+  destr_in H0. simpl in *.
+  destruct H.
+  eapply acc_strmap_acc; eauto. subst. rewrite Maps.PTree.gss. congruence.
+  eauto.
+Qed.
+
+Lemma acc_symbol_strings_in:
+  forall l idbytes i,
+    fold_right (acc_symbol_strings) (OK []) l = OK idbytes ->
+    In i l ->
+    In i (map fst idbytes).
+Proof.
+  induction l; simpl; intros; eauto. easy.
+  unfold acc_symbol_strings in H at 1. autoinv. simpl. intuition eauto.
+Qed.
+
+Lemma get_strings_map_bytes_has_mapping:
+  forall l idbytes strmap sbytes,
+    get_strings_map_bytes l = OK (idbytes, strmap, sbytes) ->
+    forall i,
+      In i l ->
+      exists si, Maps.PTree.get i strmap = Some si.
+Proof.
+  unfold get_strings_map_bytes. intros.
+  autoinv.
+  eapply acc_symbol_strings_in in EQ; eauto.
+  eapply acc_strmap_exists in EQ; eauto. destruct (Maps.PTree.get i strmap) eqn:?; try congruence.
+  eauto.
+Qed.
+
+Lemma link_symbtable_in:
+  forall s1 s2 s,
+    RelocLinking.link_symbtable s1 s2 = Some s ->
+    forall x,
+      In x s ->
+      RelocLinking.link_symb_merge (Maps.PTree.get (symbentry_id x) (symbtable_to_tree s1))
+                                   (Maps.PTree.get (symbentry_id x) (symbtable_to_tree s2)) = Some x.
+Proof.
+  intros.
+  unfold RelocLinking.link_symbtable in H. autoinv.
+  rewrite ! andb_true_iff in Heqb. intuition.
+  rewrite in_map_iff in H0.
+  destruct H0 as ((id & se) & EQ & IN). subst. simpl in *.
+  apply  Maps.PTree.elements_complete in IN.
+  rewrite Maps.PTree.gcombine in IN. 2: reflexivity.
+
+  assert (id = symbentry_id se). {
+    unfold RelocLinking.link_symb_merge in *. autoinv.
+    exploit symbtable_to_tree_get_id. apply Heqo. 
+    exploit symbtable_to_tree_get_id. apply Heqo0. intuition subst.
+    unfold RelocLinking.link_symb in H0. autoinv.
+    simpl; auto. simpl; auto.
+    exploit symbtable_to_tree_get_id. apply Heqo. intuition.
+    exploit symbtable_to_tree_get_id. apply H0. intuition.
+  }
+  subst. auto.
+Qed.
+
+Lemma update_reloctable_valid:
+  forall symt sim rtbl rtbl',
+    Forall valid_relocentry rtbl ->
+    (forall i n, Maps.PTree.get i sim = Some n -> Z.of_N n < two_p 24) ->
+    RelocLinking1.update_reloctable_symb symt sim rtbl = Some rtbl' ->
+    Forall valid_relocentry rtbl'.
+Proof.
+  intros symt sim rtbl rtbl' F LT URS.
+  unfold RelocLinking1.update_reloctable_symb in URS.
+  revert F rtbl' URS.
+  induction 1; simpl; intros; eauto. inv URS. constructor.
+  unfold RelocLinking1.acc_update_reloc_symb in URS at 1. autoinv.
+  constructor; eauto.
+  unfold RelocLinking1.update_reloc_symb in Heqo0. autoinv.
+  inv H. constructor; eauto.
+Qed.
+
+Lemma link_reloctable_valid:
+  forall sz symt1 symt2 sim rtbl1 rtbl2 rtbl,
+    Forall valid_relocentry rtbl1 ->
+    Forall valid_relocentry rtbl2 ->
+    (forall i n, Maps.PTree.get i sim = Some n -> Z.of_N n < two_p 24) ->
+    RelocLinking1.link_reloctable sz symt1 symt2 sim rtbl1 rtbl2 = Some rtbl ->
+    Forall valid_relocentry rtbl.
+Proof.
+  intros sz symt1 symt2 sim rtbl1 rtbl2 rtbl F1 F2 LT LR.
+  unfold RelocLinking1.link_reloctable in LR. autoinv.
+  rewrite Forall_forall. intros.
+  rewrite in_app in H. destruct H.
+  revert x H. rewrite <- Forall_forall. eapply update_reloctable_valid. 3: eauto. auto. auto.
+  rewrite in_map_iff in H.
+  destruct H as (x0 & SHIFT & IN).
+  exploit update_reloctable_valid. apply F2. eauto. eauto. rewrite Forall_forall.
+  intro A; specialize (A _ IN). subst.
+  inv A; constructor; simpl; auto.
+  admit.                    (* reloc offset could overflow *)
+Admitted.
+
 Instance tl : @TransfLink _ _ RelocBingenproof.linker2
                           linker2
                           match_prog.
@@ -310,4 +833,227 @@ Proof.
   erewrite decode_tables_correct; eauto.
   erewrite decode_tables_correct; eauto.
   simpl. rewrite H.
+  cut (exists tp, transf_program p = OK tp).
+  intros (tp & TP); rewrite TP; eauto.
+  unfold transf_program in *.
+  monadInv H0. monadInv H1.
+  repeat destr_in EQ0. repeat destr_in EQ2.
+  monadInv H1. monadInv H2.
+  repeat destr_in EQ2. repeat destr_in EQ4.
+
+  assert (
+      exists s0 v v0,
+        SecTable.get sec_data_id (prog_sectable p1) = Some v /\
+        SecTable.get sec_code_id (prog_sectable p1) = Some v0 /\
+        RelocLinking.reloc_symbtable (RelocLinking.reloc_offset_fun (sec_size v) (sec_size v0))
+            (prog_symbtable p2) = Some s0 /\
+      Some (prog_symbtable p) = RelocLinking.link_symbtable (prog_symbtable p1) s0).
+  {
+    clear - H.
+    unfold link_reloc_bingen in H. repeat destr_in H.
+    unfold RelocBingen.transf_program in Heqr1. monadInv Heqr1. repeat destr_in EQ2. simpl.
+    clear EQ. unfold RelocLinking1.link_reloc_prog in Heqo.
+    repeat destr_in Heqo. simpl. clear Heqo1 Heqo2. simpl in *.
+    unfold RelocLinking.link_reloc_prog in Heqo0.
+    repeat destr_in Heqo0. simpl.
+    unfold decode_prog_code_section in Heqr0, Heqr.
+    repeat destr_in Heqr0. repeat destr_in Heqr.
+    monadInv H0. monadInv H1.
+    repeat destr_in EQ0. repeat destr_in EQ3. simpl in *.
+
+
+    erewrite SecTable_gsspec in Heqo1, Heqo2. 4,7: eauto.
+    2-5: unfold sec_code_id, sec_data_id, SecTblParams.ofs; lia.
+    repeat destr_in Heqo2.
+    repeat destr_in Heqo1. inv e0. rewrite H0.
+    (do 3 eexists); (do 3 split); eauto.
+    rewrite <- Heqo4. f_equal. f_equal.
+    unfold decode_code_section in EQ2. repeat destr_in EQ2.
+    monadInv H1.
+    simpl.
+    erewrite decode_instrs'_size; eauto.
+  }
+  
+  assert (EXsz: exists z,
+             fold_right
+               (fun (id : ident) (acc : res Z) =>
+                  match acc with
+                  | OK z =>
+                    match SymbolString.find_symbol_pos id with
+                    | Some pos => OK (z + 2 + Z.of_nat (length pos))
+                    | None => Error (msg "cannot find string")
+                    end
+                  | Error _ => acc
+                  end) (OK 0) (fold_right acc_symbols [] (prog_symbtable p)) = OK z
+             /\ z < Int.max_unsigned
+         ).
+  {
+    clear - H. unfold link_reloc_bingen in H. repeat destr_in H.
+    unfold RelocBingen.transf_program in Heqr1. autoinv. eexists; split; eauto.
+  }
+  destruct EXsz as (sz & EQsz & LT).
+  exploit (get_strings_map_bytes_exists (prog_symbtable p)); eauto.
+  intros (idbytes & strmap & sbytes & smb). rewrite smb. simpl.
+  destruct H0 as (s0 & v & v0 & GETdata & GETcode & RELOCsym & EQsym).
+
+  assert (NRsymb_id:   list_norepet (map symbentry_id (prog_symbtable p))).
+  {
+    clear - EQsym. symmetry in EQsym.
+    unfold RelocLinking.link_symbtable in EQsym.
+    repeat destr_in EQsym.
+    rewrite map_map.
+    rewrite list_map_exten with (f:= fst).
+    apply Maps.PTree.elements_keys_norepet.
+    intros.
+    destruct x.
+    apply Maps.PTree.elements_complete in H.
+    rewrite Maps.PTree.gcombine in H by reflexivity. simpl.
+    unfold RelocLinking.link_symb_merge in H.
+      assert (LinkSymbId:
+                forall s1 s2 s3,
+                       RelocLinking.link_symb s1 s2 = Some s3 ->
+                       symbentry_id s1 = symbentry_id s3 /\
+                       symbentry_id s2 = symbentry_id s3
+             ).
+      {
+        unfold RelocLinking.link_symb. clear. intros. autoinv; simpl; intuition.
+      }
+      autoinv; repeat
+                 match goal with
+                   H: Maps.PTree.get _ (symbtable_to_tree _) = _ |- _ =>
+                   apply symbtable_to_tree_get_id in H
+                 | H: RelocLinking.link_symb _ _ = Some _ |- _ =>
+                   apply LinkSymbId in H
+                 end; intuition congruence.
+  }
+
+  assert (valid_strtable idbytes strmap).
+  {
+    generalize smb; intro smb'.
+    unfold get_strings_map_bytes in smb. monadInv smb.
+    exploit gsmb_valid_strtable. apply smb'. eauto. eauto.
+    repeat destr_in EQ4.
+  }
+
+  assert (Valids: Forall (valid_symbentry strmap) (prog_symbtable p)).
+  {
+    rewrite Forall_forall. intros.
+
+
+
+    exploit link_symbtable_in. 2: eauto. eauto.
+
+    assert (ValidRelocSymbentries: Forall (valid_symbentry t0) s0).
+    {
+      clear - f1 RELOCsym.
+      unfold RelocLinking.reloc_symbtable in RELOCsym.
+      revert f1 RELOCsym.
+      generalize (prog_symbtable p2) (RelocLinking.reloc_offset_fun (sec_size v) (sec_size v0)) s0. clear.
+      induction s; simpl; intros; eauto. inv RELOCsym; auto.
+      inv f1.
+      unfold RelocLinking.reloc_iter at 1 in RELOCsym.
+      autoinv.
+      constructor; eauto.
+      unfold RelocLinking.reloc_symbol in Heqo1. autoinv.
+      inv H1. rewrite Heqs0 in *. constructor; simpl in *; auto.
+      admit.                    (* symbentry_value relocated could overflow... *)
+    }
+    
+
+    unfold RelocLinking.link_symb_merge. destr.
+
+    destr.
+    Lemma acc_symbols_map:
+      forall l,
+        fold_right acc_symbols [] l = map symbentry_id l.
+    Proof.
+      induction l; simpl; intros; eauto.
+    Qed.
+    - exploit symbtable_to_tree_get_id. apply Heqo.
+      exploit symbtable_to_tree_get_id. apply Heqo0.
+      intros (EQid1 & IN1) (EQid2 & IN2) LS.
+      rewrite Forall_forall in f. generalize (f _ IN2).
+      rewrite Forall_forall in ValidRelocSymbentries. generalize (ValidRelocSymbentries _ IN1).
+      unfold RelocLinking.link_symb in LS.
+      inversion 1; inversion 1; constructor; simpl; eauto.
+      + autoinv; simpl; auto.
+        rewrite Zmax_spec; destr; vm_compute; intuition congruence.
+        vm_compute; intuition congruence.
+      + autoinv; simpl; auto.
+        vm_compute; intuition congruence.
+        vm_compute; intuition congruence.
+      + edestruct get_strings_map_bytes_has_mapping as (si & MAP1).
+        3: rewrite MAP1. eauto.
+        rewrite acc_symbols_map. rewrite in_map_iff.
+        eexists; split; eauto. eexists; split; eauto.
+        destruct H0 as (o & V & LT'). destruct V. eapply table_range; eauto.
+      + autoinv; simpl; auto.
+    - intro A; inv A.
+      exploit symbtable_to_tree_get_id. apply Heqo.
+      intros (EQid1 & IN1).
+      rewrite Forall_forall in f. generalize (f _ IN1).
+      inversion 1; constructor; simpl; eauto.
+      edestruct get_strings_map_bytes_has_mapping as (si & MAP1).
+      3: rewrite MAP1. eauto.
+      rewrite acc_symbols_map. rewrite in_map_iff.
+      eauto. eexists; split; eauto.
+      destruct H0 as (o & V & LT'). destruct V. eapply table_range; eauto.
+    - intro A.
+      exploit symbtable_to_tree_get_id. apply A.
+      intros (EQid1 & IN1).
+      rewrite Forall_forall in ValidRelocSymbentries. generalize (ValidRelocSymbentries _ IN1).
+      inversion 1; constructor; simpl; eauto.
+      edestruct get_strings_map_bytes_has_mapping as (si & MAP1).
+      3: rewrite MAP1. eauto.
+      rewrite acc_symbols_map. rewrite in_map_iff.
+      eauto. eexists; split; eauto.
+      destruct H0 as (o & V & LT'). destruct V. eapply table_range; eauto.
+  }
+  rewrite pred_dec_true by auto.
+  assert (prog_strtable p = Maps.PTree.empty Z).
+  {
+    clear - e e0 H.
+    unfold link_reloc_bingen in H. autoinv.
+    unfold RelocBingen.transf_program in Heqr1. autoinv. simpl. clear - e e0 Heqo Heqr Heqr0.
+    unfold RelocLinking1.link_reloc_prog in Heqo. autoinv. simpl.
+    clear Heqo1 Heqo2.
+    unfold RelocLinking.link_reloc_prog in Heqo0. autoinv. simpl.
+    clear Heqo5 Heqo4 Heqo1 Heqo2 Heqo3.
+    unfold decode_prog_code_section in Heqr. autoinv. simpl. auto.
+  }
+  rewrite pred_dec_true by auto.
+  rewrite pred_dec_true by auto.
+  assert ((forall id : reloctable_id, Forall valid_relocentry (get_reloctable id (prog_reloctables p)))).
+  {
+    clear - f2 f0 H.
+    unfold link_reloc_bingen in H. autoinv.
+    unfold RelocBingen.transf_program in Heqr1. autoinv. simpl.
+    clear EQ1 EQ l.
+    unfold RelocLinking1.link_reloc_prog in Heqo. autoinv. simpl. clear Heqo0.
+    unfold RelocLinking1.link_data_reloctable in Heqo1. autoinv.
+    unfold RelocLinking1.link_code_reloctable in Heqo2. autoinv.
+    unfold decode_prog_code_section in Heqr, Heqr0. autoinv. simpl in *.
+    clear - H0 H1 f0 f2.
+    intros.
+    
+    specialize (f0 id). specialize (f2 id).
+    destruct id; simpl in *; eapply link_reloctable_valid. 4,8: eauto. all: eauto.
+    admit.
+    admit.                      (* sim gives values < 2 ^ 24 *)
+  }
+  rewrite pred_dec_true by auto.
+
+  exploit create_symbtable_section_succeeds.
+  2: intros (symsec & CSS); rewrite CSS.
+  {
+    rewrite Forall_forall. intros xx IN.
+    exploit link_symbtable_in. eauto. eauto.
+    intros.
+    eapply get_strings_map_bytes_has_mapping. eauto.
+    rewrite acc_symbols_map.
+    apply in_map. auto.
+  }
+  simpl. rewrite app_length. simpl.
+
+  erewrite link_reloc_bingen_sectable; eauto. simpl. eauto.
 Admitted.
